Cslib/Computability/Machines/MultiTapeTuring/Routines/Typed.lean
@@ -1,0 +1,54 @@
+/-
+Copyright (c) 2026 Christian Reitwiessner. All rights reserved.
+Released under Apache 2.0 license as described in the file LICENSE.
+Authors: Christian Reitwiessner
+-/
+
+module
+
+public import Cslib.Computability.Machines.MultiTapeTuring.Encoding
+public import Cslib.Computability.Machines.MultiTapeTuring.StructuralMachines
+
+namespace Turing
+namespace Routines
+
+/-- Turing machine `tm` computes a function on data from tape `i` and updates tape `j`. -/
+-- TODO move this somewhere else
+public def computes_function {k : ℕ}
+  (tm : MultiTapeTM k Char) (f : TapeView → Data → TapeView)
+  (i j : Fin k) (_h_neq : i ≠ j)
+  (views : Fin k → TapeView) :=
+  tm.eval_struct views = some (Function.update views j
+    (((views i).current.map (f (views j))).getD (views j)))
+
+-- TODO could generalize this to `f` having a preimage β.
+public def computes_function_push {k : ℕ}
+  {α : Type} [StrEnc α]
+  (tm : MultiTapeTM k Char) (f : Data → α)
+  (i j : Fin k) (_h_neq : i ≠ j) :=
+  computes_function tm (fun tv d => tv.pushList (StrEnc.toData (f d))) i j _h_neq
+
+/-- Turing machine `tm` computes a function of the current item at tape `i` seen as type
+-- `α` and pushes the result (type `β`) to tape `j`. -/
+-- public def computes_function_push' {k : ℕ}
+--   {α β : Type} [StrEnc α] [StrEnc β]
+--   (tm : MultiTapeTM k Char) (f : α → β)
+--   (i j : Fin k) (_h_neq : i ≠ j) :=
+--   computes_function tm (fun tv d => tv.pushList (StrEnc.toData (f d))) i j _h_neq
+
+public def computes_function_push_bool {k : ℕ}
+  (tm : MultiTapeTM k Char) (f : Data → Bool)
+  (i j : Fin k) (h_neq : i ≠ j) :=
+  computes_function_push (α := Bool) tm f i j h_neq
+
+/-- Turing machine `tm` updates the head of tape `i`. -/
+public def computes_function_update {k : ℕ}
+  {α β : Type} [StrEnc α] [StrEnc β]
+  (tm : MultiTapeTM k Char) (f : α → β)
+  (i : Fin k)
+  (views : Fin k → TapeView) :=
+  tm.eval_struct views = some (Function.update views i ((views i).updateListHeadTyped f))
+
+
+end Routines
+end Turing
